Starting integrating new typing of global_env (by Sim) into PCUIC
In particular renaming:
- global_declarations  ->  global_env
- global_context  ->  global_context_ext
- universe_context  ->  universes_decl
- consistent_universe_context_instance  ->  consistent_instance_ext
- snd Σ  ->  global_ext_constraints Σ
- on_global_decls_impl  ->  on_global_env_impl

pcuic/theories/PCUICTyping.v
@@ -20,10 +20,6 @@ Set Asymmetric Patterns.
 
  *)
 
-(** Use a coercion for this common projection of the global context. *)
-Definition fst_ctx : global_context -> global_declarations := fst.
-Coercion fst_ctx : global_context >-> global_declarations.
-
 Definition isSort T :=
   match T with
   | tSort u => True
@@ -56,7 +52,7 @@ Definition global_decl_ident d :=
   | InductiveDecl id _ => id
   end.
 
-Fixpoint lookup_env (Σ : global_declarations) (id : ident) : option global_decl :=
+Fixpoint lookup_env (Σ : global_env) (id : ident) : option global_decl :=
   match Σ with
   | nil => None
   | hd :: tl =>
@@ -64,7 +60,7 @@ Fixpoint lookup_env (Σ : global_declarations) (id : ident) : option global_decl
     else lookup_env tl id
   end.
 
-Definition declared_constant (Σ : global_declarations) (id : ident) decl : Prop :=
+Definition declared_constant (Σ : global_env) (id : ident) decl : Prop :=
   lookup_env Σ id = Some (ConstantDecl id decl).
 
 Definition declared_minductive Σ mind decl :=
@@ -82,6 +78,7 @@ Definition declared_projection Σ mdecl idecl (proj : projection) pdecl : Prop :
   declared_inductive Σ mdecl (fst (fst proj)) idecl /\
   List.nth_error idecl.(ind_projs) (snd proj) = Some pdecl /\
   mdecl.(ind_npars) = snd (fst proj).
+
 
 (** Inductive substitution, to produce a constructors' type *)
 Definition inds ind u (l : list one_inductive_body) :=
@@ -181,7 +178,7 @@ Definition iota_red npar c args brs :=
 Local Open Scope type_scope.
 Arguments OnOne2 {A} P%type l l'.
 
-Inductive red1 (Σ : global_declarations) (Γ : context) : term -> term -> Type :=
+Inductive red1 (Σ : global_env) (Γ : context) : term -> term -> Type :=
 (** Reductions *)
 (** Beta *)
 | red_beta na t b a :
@@ -239,6 +236,7 @@ Inductive red1 (Σ : global_declarations) (Γ : context) : term -> term -> Type 
     nth_error args (pars + narg) = Some arg ->
     red1 Σ Γ (tProj (i, pars, narg) (mkApps (tConstruct i k u) args)) arg
 
+
 | abs_red_l na M M' N : red1 Σ Γ M M' -> red1 Σ Γ (tLambda na M N) (tLambda na M' N)
 | abs_red_r na M M' N : red1 Σ (Γ ,, vass na N) M M' -> red1 Σ Γ (tLambda na N M) (tLambda na N M')
 
@@ -279,7 +277,7 @@ Inductive red1 (Σ : global_declarations) (Γ : context) : term -> term -> Type 
     red1 Σ Γ (tCoFix mfix0 idx) (tCoFix mfix1 idx).
 
 Lemma red1_ind_all :
-  forall (Σ : global_declarations) (P : context -> term -> term -> Type),
+  forall (Σ : global_env) (P : context -> term -> term -> Type),
 
        (forall (Γ : context) (na : name) (t b a : term),
         P Γ (tApp (tLambda na t b) a) (b {0 := a})) ->
@@ -601,30 +599,100 @@ Definition types_of_case ind mdecl idecl params u p pty :=
   | None => None
   end.
 
+Definition on_udecl_decl {A} (F : universes_decl -> A) d : A :=
+  match d with
+  | ConstantDecl  _ cb => F cb.(cst_universes)
+  | InductiveDecl _ mb => F mb.(ind_universes)
+  end.
+
+Definition monomorphic_udecl u :=
+  match u with
+  | Monomorphic_ctx ctx => ctx
+  | _ => ContextSet.empty
+  end.
+
+Definition monomorphic_udecl_decl := on_udecl_decl monomorphic_udecl.
+
+Definition monomorphic_levels_decl := fst ∘ monomorphic_udecl_decl.
+
+Definition monomorphic_constraints_decl := snd ∘ monomorphic_udecl_decl.
+
+Definition levels_of_udecl u :=
+  match u with
+  | Monomorphic_ctx ctx => fst ctx
+  | Polymorphic_ctx ctx
+  | Cumulative_ctx (ctx, _) => AUContext.levels ctx
+  end.
+
+Definition constraints_of_udecl u :=
+  match u with
+  | Monomorphic_ctx ctx => snd ctx
+  | Polymorphic_ctx ctx
+  | Cumulative_ctx (ctx, _) => snd (AUContext.repr ctx)
+  end.
+
+Definition universes_decl_of_decl := on_udecl_decl (fun x => x).
+
+(* Definition LevelSet_add_list l := LevelSet.union (LevelSetProp.of_list l). *)
+
+Definition LevelSet_pair x y
+  := LevelSet.add y (LevelSet.singleton x).
+
+
+Definition global_levels (Σ : global_env) : LevelSet.t
+  := fold_right (fun decl lvls => LevelSet.union (monomorphic_levels_decl decl) lvls)
+                (LevelSet_pair Level.lSet Level.lProp) Σ.
+
+Definition global_constraints (Σ : global_env) : constraints
+  := fold_right (fun decl ctrs => ConstraintSet.union
+                                (monomorphic_constraints_decl decl) ctrs)
+               ConstraintSet.empty Σ.
+
+Definition global_ext_levels (Σ : global_env_ext) : LevelSet.t
+  := LevelSet.union (levels_of_udecl (snd Σ)) (global_levels Σ.1).
+
+Definition global_ext_constraints (Σ : global_env_ext) : constraints
+  := ConstraintSet.union (constraints_of_udecl (snd Σ))
+                         (global_constraints Σ.1).
+
+
+Lemma prop_global_ext_levels Σ : LevelSet.In Level.prop (global_ext_levels Σ).
+Proof.
+  destruct Σ as [Σ φ]; cbn.
+  apply LevelSetFact.union_3. cbn -[global_levels]; clear φ.
+  induction Σ.
+  - cbn. now apply LevelSetFact.add_1.
+  - simpl. now apply LevelSetFact.union_3.
+Qed.
+
+
 (** Check that [uctx] instantiated at [u] is consistent with the current universe graph. *)
 
-Definition consistent_universe_context_instance `{checker_flags}
-           (φ : constraints) uctx u :=
+Definition consistent_instance `{checker_flags} (φ : constraints) uctx (u : universe_instance) :=
   match uctx with
-  | Monomorphic_ctx c => True
+  | Monomorphic_ctx c => List.length u = 0
   | Polymorphic_ctx c
-  | Cumulative_ctx (c, _) =>
-    let '(inst, cstrs) := UContext.dest c in
-    List.length inst = List.length u /\
-    consistent (ConstraintSet.union (subst_instance_cstrs u cstrs) φ)
+  | Cumulative_ctx (c, _) => (* FIXME Cumulative *)
+    let '(inst, cstrs) := AUContext.repr c in
+    List.length u = List.length inst /\
+    valid_constraints φ (subst_instance_cstrs u cstrs)
   end.
+
+Definition consistent_instance_ext `{checker_flags}
+  := consistent_instance ∘ global_ext_constraints.
+
 
 Reserved Notation " Σ ;;; Γ |- t : T " (at level 50, Γ, t, T at next level).
 Reserved Notation " Σ ;;; Γ |- t <= u " (at level 50, Γ, t, u at next level).
 
 (** ** Cumulativity *)
 
-Inductive cumul `{checker_flags} (Σ : global_context) (Γ : context) : term -> term -> Type :=
-| cumul_refl t u : leq_term (snd Σ) t u -> Σ ;;; Γ |- t <= u
-| cumul_red_l t u v : red1 (fst Σ) Γ t v -> Σ ;;; Γ |- v <= u -> Σ ;;; Γ |- t <= u
-| cumul_red_r t u v : Σ ;;; Γ |- t <= v -> red1 (fst Σ) Γ u v -> Σ ;;; Γ |- t <= u
+Inductive cumul `{checker_flags} (Σ : global_env_ext) (Γ : context) : term -> term -> Type :=
+| cumul_refl t u : leq_term (global_ext_constraints Σ) t u -> Σ ;;; Γ |- t <= u
+| cumul_red_l t u v : red1 Σ.1 Γ t v -> Σ ;;; Γ |- v <= u -> Σ ;;; Γ |- t <= u
+| cumul_red_r t u v : Σ ;;; Γ |- t <= v -> red1 Σ.1 Γ u v -> Σ ;;; Γ |- t <= u
 
-where " Σ ;;; Γ |- t <= u " := (@cumul _ Σ Γ t u) : type_scope.
+where " Σ ;;; Γ |- t <= u " := (cumul Σ Γ t u) : type_scope.
 
 (** *** Conversion
 
@@ -634,7 +702,7 @@ where " Σ ;;; Γ |- t <= u " := (@cumul _ Σ Γ t u) : type_scope.
 Definition conv `{checker_flags} Σ Γ T U : Type :=
   (Σ ;;; Γ |- T <= U) * (Σ ;;; Γ |- U <= T).
 
-Notation " Σ ;;; Γ |- t = u " := (@conv _ Σ Γ t u) (at level 50, Γ, t, u at next level) : type_scope.
+Notation " Σ ;;; Γ |- t = u " := (conv Σ Γ t u) (at level 50, Γ, t, u at next level) : type_scope.
 
 Axiom conv_refl : forall `{checker_flags} Σ Γ t, Σ ;;; Γ |- t = t.
 Axiom cumul_refl' : forall `{checker_flags} Σ Γ t, Σ ;;; Γ |- t <= t. (* easy *)
@@ -690,8 +758,8 @@ End TypeLocal.
 
 (** Well-formedness of local environments embeds a sorting for each variable *)
 
-Definition lift_typing (P : global_context -> context -> term -> term -> Type) :
-  (global_context -> context -> term -> option term -> Type) :=
+Definition lift_typing (P : global_env_ext -> context -> term -> term -> Type) :
+  (global_env_ext -> context -> term -> option term -> Type) :=
   fun Σ Γ t T =>
     match T with
     | Some T => P Σ Γ t T
@@ -705,12 +773,12 @@ Definition on_local_decl (P : context -> term -> option term -> Type) Γ d :=
   end.
 
 Section TypeLocalOver.
-  Context (typing : forall (Σ : global_context) (Γ : context), term -> term -> Type).
-  Context (property : forall (Σ : global_context) (Γ : context),
+  Context (typing : forall (Σ : global_env_ext) (Γ : context), term -> term -> Type).
+  Context (property : forall (Σ : global_env_ext) (Γ : context),
               All_local_env (lift_typing typing Σ) Γ ->
               forall (t T : term), typing Σ Γ t T -> Type).
 
-  Inductive All_local_env_over (Σ : global_context) :
+  Inductive All_local_env_over (Σ : global_env_ext) :
     forall (Γ : context), All_local_env (lift_typing typing Σ) Γ -> Type :=
   | localenv_over_nil :
       All_local_env_over Σ [] (localenv_nil _)
@@ -734,12 +802,12 @@ Section TypeLocalOver.
 End TypeLocalOver.
 
 Section WfArity.
-  Context (typing : forall (Σ : global_context) (Γ : context), term -> term -> Type).
+  Context (typing : forall (Σ : global_env_ext) (Γ : context), term -> term -> Type).
 
   Definition isWfArity Σ (Γ : context) T :=
     { ctx & { s & (destArity [] T = Some (ctx, s)) * All_local_env (lift_typing typing Σ) (Γ ,,, ctx) } }.
 
-  Context (property : forall (Σ : global_context) (Γ : context),
+  Context (property : forall (Σ : global_env_ext) (Γ : context),
               All_local_env (lift_typing typing Σ) Γ ->
               forall (t T : term), typing Σ Γ t T -> Type).
 
@@ -747,7 +815,7 @@ Section WfArity.
     { wfa : isWfArity Σ Γ T & All_local_env_over typing property Σ _ (snd (projT2 (projT2 wfa))) }.
 End WfArity.
 
-Inductive typing `{checker_flags} (Σ : global_context) (Γ : context) : term -> term -> Type :=
+Inductive typing `{checker_flags} (Σ : global_env_ext) (Γ : context) : term -> term -> Type :=
 | type_Rel n decl :
     All_local_env (lift_typing typing Σ) Γ ->
     nth_error Γ n = Some decl ->
@@ -755,12 +823,8 @@ Inductive typing `{checker_flags} (Σ : global_context) (Γ : context) : term ->
 
 | type_Sort l :
     All_local_env (lift_typing typing Σ) Γ ->
+    LevelSet.In l (global_ext_levels Σ) ->
     Σ ;;; Γ |- tSort (Universe.make l) : tSort (Universe.super l)
-
-(* | type_Cast c k t s : *)
-(*     Σ ;;; Γ |- t : tSort s -> *)
-(*     Σ ;;; Γ |- c : t -> *)
-(*     Σ ;;; Γ |- (tCast c k t) : t *)
 
 | type_Prod na A B s1 s2 :
     Σ ;;; Γ |- A : tSort s1 ->
@@ -785,36 +849,36 @@ Inductive typing `{checker_flags} (Σ : global_context) (Γ : context) : term ->
 
 | type_Const cst u :
     All_local_env (lift_typing typing Σ) Γ ->
-    forall decl (isdecl : declared_constant (fst Σ) cst decl),
-    consistent_universe_context_instance (snd Σ) decl.(cst_universes) u ->
+    forall decl (isdecl : declared_constant Σ.1 cst decl),
+    consistent_instance_ext Σ decl.(cst_universes) u ->
     Σ ;;; Γ |- (tConst cst u) : subst_instance_constr u decl.(cst_type)
 
 | type_Ind ind u :
     All_local_env (lift_typing typing Σ) Γ ->
-    forall mdecl idecl (isdecl : declared_inductive (fst Σ) mdecl ind idecl),
-    consistent_universe_context_instance (snd Σ) mdecl.(ind_universes) u ->
+    forall mdecl idecl (isdecl : declared_inductive Σ.1 mdecl ind idecl),
+    consistent_instance_ext Σ mdecl.(ind_universes) u ->
     Σ ;;; Γ |- (tInd ind u) : subst_instance_constr u idecl.(ind_type)
 
 | type_Construct ind i u :
     All_local_env (lift_typing typing Σ) Γ ->
-    forall mdecl idecl cdecl (isdecl : declared_constructor (fst Σ) mdecl idecl (ind, i) cdecl),
-    consistent_universe_context_instance (snd Σ) mdecl.(ind_universes) u ->
+    forall mdecl idecl cdecl (isdecl : declared_constructor Σ.1 mdecl idecl (ind, i) cdecl),
+    consistent_instance_ext Σ mdecl.(ind_universes) u ->
     Σ ;;; Γ |- (tConstruct ind i u) : type_of_constructor mdecl cdecl (ind, i) u
 
 | type_Case ind u npar p c brs args :
-    forall mdecl idecl (isdecl : declared_inductive (fst Σ) mdecl ind idecl),
+    forall mdecl idecl (isdecl : declared_inductive Σ.1 mdecl ind idecl),
     mdecl.(ind_npars) = npar ->
     let pars := List.firstn npar args in
     forall pty, Σ ;;; Γ |- p : pty ->
     forall indctx pctx ps btys, types_of_case ind mdecl idecl pars u p pty = Some (indctx, pctx, ps, btys) ->
-    check_correct_arity (snd Σ) idecl ind u indctx pars pctx ->
+    check_correct_arity (global_ext_constraints Σ) idecl ind u indctx pars pctx ->
     List.Exists (fun sf => universe_family ps = sf) idecl.(ind_kelim) ->
     Σ ;;; Γ |- c : mkApps (tInd ind u) args ->
     All2 (fun x y => (fst x = fst y) * (Σ ;;; Γ |- snd x : snd y)) brs btys ->
     Σ ;;; Γ |- tCase (ind, npar) p c brs : mkApps p (List.skipn npar args ++ [c])
 
 | type_Proj p c u :
-    forall mdecl idecl pdecl (isdecl : declared_projection (fst Σ) mdecl idecl p pdecl) args,
+    forall mdecl idecl pdecl (isdecl : declared_projection Σ.1 mdecl idecl p pdecl) args,
     Σ ;;; Γ |- c : mkApps (tInd (fst (fst p)) u) args ->
     (** Actually ensured by typing + validity, but necessary for weakening and substitution. *)
     #|args| = ind_npars mdecl ->
@@ -850,48 +914,28 @@ where " Σ ;;; Γ |- t : T " := (@typing _ Σ Γ t T) : type_scope.
 
 (** ** Typechecking of global environments *)
 
-Definition add_global_constraints (uctx : universe_context) (G : constraints) : constraints
-  := match uctx with
-     | Monomorphic_ctx (inst, cstrs) =>
-       ConstraintSet.union cstrs G
-     | Polymorphic_ctx _ => G
-     | Cumulative_ctx _ => G
-     end.
 
-Definition add_global_decl (decl : global_decl) (Σ : global_context) :=
-  let univs := match decl with
-               | ConstantDecl _ d => d.(cst_universes)
-               | InductiveDecl _ d => d.(ind_universes)
-               end
-  in (decl :: fst Σ, add_global_constraints univs (snd Σ)).
-
-Definition add_global_declarations (Σ : global_declarations) init : global_context
-  := List.fold_left (fun Σ d => add_global_decl d Σ) Σ init.
-
-Definition reconstruct_global_context Σ
-  := add_global_declarations Σ ([], ConstraintSet.empty).
-
-Definition isType `{checker_flags} (Σ : global_context) (Γ : context) (t : term) :=
+Definition isType `{checker_flags} (Σ : global_env_ext) (Γ : context) (t : term) :=
   { s : _ & Σ ;;; Γ |- t : tSort s }.
 
 Definition has_nparams npars ty :=
   decompose_prod_n_assum [] npars ty <> None.
 
-Definition unlift_opt_pred (P : global_context -> context -> option term -> term -> Type) :
-  (global_context -> context -> term -> term -> Type) :=
+Definition unlift_opt_pred (P : global_env_ext -> context -> option term -> term -> Type) :
+  (global_env_ext -> context -> term -> term -> Type) :=
   fun Σ Γ t T => P Σ Γ (Some t) T.
 
 (** *** Typing of inductive declarations *)
 
 Section GlobalMaps.
   Context {cf: checker_flags}.
-  Context (P : global_context -> context -> term -> option term -> Type).
+  Context (P : global_env_ext -> context -> term -> option term -> Type).
 
   Section TypeCtx.
 
     (** For well-formedness of inductive declarations we need a way to check that a given
         context is typable in [Prop]. *)
-    Context (Σ : global_context) (Γ : context).
+    Context (Σ : global_env_ext) (Γ : context).
 
     Fixpoint type_local_ctx (Δ : context) (u : universe) : Type :=
       match Δ with
@@ -924,7 +968,7 @@ Section GlobalMaps.
   Arguments cshape_args {mdecl i idecl cdecl}.
   Arguments cshape_args_univ {mdecl i idecl cdecl}.
 
-  Definition on_constructor (Σ : global_context) (mind : kername)
+  Definition on_constructor (Σ : global_env_ext) (mind : kername)
              (mdecl : mutual_inductive_body)
              (i : nat) (idecl : one_inductive_body)
              (c : nat) (cdecl : ident * term * nat) : Type :=
@@ -934,13 +978,13 @@ Section GlobalMaps.
            type_local_ctx Σ (arities_context mdecl.(ind_bodies) ,,, mdecl.(ind_params))
                           cs.(cshape_args) cs.(cshape_args_univ) }.
 
-  Definition on_constructors (Σ : global_context) mind mdecl i idecl l :=
+  Definition on_constructors (Σ : global_env_ext) mind mdecl i idecl l :=
     Alli (on_constructor Σ mind mdecl i idecl) 0 l.
 
   (** Projections have their parameter context smashed to avoid costly computations
       during type-checking. *)
 
-  Definition on_projection (Σ : global_context) mind mdecl (i : nat) (idecl : one_inductive_body)
+  Definition on_projection (Σ : global_env_ext) mind mdecl (i : nat) (idecl : one_inductive_body)
              (k : nat) (p : ident * term) :=
     let ctx := smash_context [] mdecl.(ind_params) in
     let Γ := ctx,, vass (nNamed idecl.(ind_name))
@@ -948,7 +992,7 @@ Section GlobalMaps.
                         (to_extended_list ctx))
     in on_type Σ Γ (snd p).
 
-  Record on_projections (Σ : global_context) mind mdecl i idecl (ictx : context) (l : list (ident * term)) : Type :=
+  Record on_projections (Σ : global_env_ext) mind mdecl i idecl (ictx : context) (l : list (ident * term)) : Type :=
     { on_projs_record : #|idecl.(ind_ctors)| = 1;
       (** The inductive must be a record *)
       on_projs_noidx : #|ictx| = 0;
@@ -978,7 +1022,7 @@ Section GlobalMaps.
     end.
 
   Section CheckSmaller.
-    Context {Σ : global_context} {mind : kername} {mdecl : mutual_inductive_body}
+    Context {Σ : global_env_ext} {mind : kername} {mdecl : mutual_inductive_body}
             {i : nat} {idecl : one_inductive_body} (indu : universe).
 
     Fixpoint check_constructors_smaller {k cstrs}
@@ -989,7 +1033,7 @@ Section GlobalMaps.
         (* The constructor's arguments bounding universe. *)
         let cstru := cshape_args_univ (snd onc).π1 in
         (* Just check it is smaller and continue *)
-        leq_universe (snd Σ) cstru indu /\ check_constructors_smaller cstrs
+        leq_universe (global_ext_constraints Σ) cstru indu /\ check_constructors_smaller cstrs
       end.
   End CheckSmaller.
 
@@ -1024,7 +1068,7 @@ Section GlobalMaps.
     end.
 
   Record on_ind_body
-         (Σ : global_context) (mind : kername) mdecl (i : nat) idecl :=
+         (Σ : global_env_ext) (mind : kername) mdecl (i : nat) idecl :=
     { (** The type of the inductive must be an arity, sharing the same params
           as the rest of the block, and maybe having a contexxt of indices. *)
       ind_indices : context; ind_sort : universe;
@@ -1075,19 +1119,46 @@ Section GlobalMaps.
 
   (** Well-formed global environments have no name clash. *)
 
-  Definition fresh_global (s : string) : global_declarations -> Prop :=
+  Definition fresh_global (s : string) : global_env -> Prop :=
     Forall (fun g => global_decl_ident g <> s).
 
-  Inductive on_global_decls φ : global_declarations -> Type :=
-  | globenv_nil : consistent φ -> on_global_decls φ []
-  | globenv_decl Σ d :
-      on_global_decls φ Σ ->
-      fresh_global (global_decl_ident d) Σ ->
-      on_global_decl (Σ, φ) d ->
-      on_global_decls φ (d :: Σ).
+  Definition satisfiable_udecl Σ φ
+    := consistent (global_ext_constraints (Σ, φ)).
 
-  Definition on_global_env (g : global_context) :=
-    on_global_decls (snd g) (fst g).
+  (* Check that: *)
+  (*   - declared levels are fresh *)
+  (*   - all levels used in constraints are declared *)
+  (*   - level used in monomorphic contexts are only monomorphic *)
+  Definition on_udecl Σ (udecl : universes_decl)
+    := let levels := levels_of_udecl udecl in
+       let global_levels := global_levels Σ in
+       let all_levels := LevelSet.union levels global_levels in
+       LevelSet.For_all (fun l => ~ LevelSet.In l global_levels) levels
+       /\ ConstraintSet.For_all (fun '(l1,_,l2) => LevelSet.In l1 all_levels
+                                               /\ LevelSet.In l2 all_levels)
+                               (constraints_of_udecl udecl)
+       /\ match udecl with
+         | Monomorphic_ctx ctx =>  LevelSet.For_all (fun l => match l with
+                                                          | Level.Var _ => false
+                                                          | _ => true
+                                                          end) (fst ctx)
+         | _ => True
+         end
+       /\ satisfiable_udecl Σ udecl.
+
+
+  Inductive on_global_env : global_env -> Type :=
+  | globenv_nil : on_global_env []
+  | globenv_decl Σ d :
+      on_global_env Σ ->
+      fresh_global (global_decl_ident d) Σ ->
+      let udecl := universes_decl_of_decl d in
+      on_udecl Σ udecl ->
+      on_global_decl (Σ, udecl) d ->
+      on_global_env (Σ ,, d).
+
+  Definition on_global_env_ext (g : global_env_ext) :=
+    on_global_env (fst g) × on_udecl (fst g) (snd g).
 
 End GlobalMaps.
 
@@ -1101,7 +1172,7 @@ Arguments onConstructors {_ P Σ mind mdecl i idecl}.
 Arguments onProjections {_ P Σ mind mdecl i idecl}.
 Arguments ind_sorts {_ P Σ mind mdecl i idecl}.
 
-(* Definition sort_irrelevant (P : global_context -> context -> option term -> term -> Type) := *)
+(* Definition sort_irrelevant (P : global_env_ext -> context -> option term -> term -> Type) := *)
 (*   forall Σ Γ b s s', P Σ Γ b (tSort s) -> P Σ Γ b (tSort s'). *)
 
 Lemma All_local_env_impl `{checker_flags} (P Q : context -> term -> option term -> Type) l :
@@ -1168,7 +1239,7 @@ Proof.
   intros. induction X; simpl; constructor; auto.
 Defined.
 
-Lemma type_local_ctx_impl (P Q : global_context -> context -> term -> option term -> Type) Σ Γ Δ u :
+Lemma type_local_ctx_impl (P Q : global_env_ext -> context -> term -> option term -> Type) Σ Γ Δ u :
   type_local_ctx P Σ Γ Δ u ->
   (forall Γ t T, P Σ Γ t T -> Q Σ Γ t T) ->
   type_local_ctx Q Σ Γ Δ u.
@@ -1178,10 +1249,37 @@ Proof.
   intros. intuition auto.
 Qed.
 
-Lemma on_global_decls_impl `{checker_flags} Σ P Q :
-  (forall Σ Γ t T, on_global_env P Σ -> P Σ Γ t T -> Q Σ Γ t T) ->
+Lemma on_global_env_impl `{checker_flags} Σ P Q :
+  (forall Σ Γ t T, on_global_env P Σ.1 -> P Σ Γ t T -> Q Σ Γ t T) ->
   on_global_env P Σ -> on_global_env Q Σ.
 Proof.
+  intros X X0.
+  simpl in *. induction X0; constructor; auto.
+  clear IHX0. destruct d; simpl.
+  - destruct c; simpl. destruct cst_body; simpl in *.
+    red in o |- *. simpl in *. now eapply X.
+    red in o |- *. simpl in *. now eapply X.
+  - red in o. simpl in *.
+    destruct o0 as [onI onP onNP].
+    constructor; auto.
+    -- eapply Alli_impl. exact onI. eauto. intros.
+       destruct x; simpl in *.
+       constructor; red; simpl.
+       --- apply onArity in X1. unfold on_arity, on_type in *; simpl in *.
+           split. now eapply X. easy.
+       --- apply onConstructors in X1. red in X1. unfold on_constructor, on_type in *. eapply Alli_impl; eauto.
+           simpl. intros. split. now eapply X. easy.
+       --- apply onProjections in X1. simpl in *.
+           unfold on_projections in *. eapply Alli_impl; intuition eauto. clear X1.
+           unfold on_projection in *; simpl in *.
+           destruct decompose_prod_assum. unfold on_type in *; eauto.
+           split. now eapply X. easy.
+    -- red in onP. red.
+       eapply All_local_env_impl. eauto.
+       intros. red in X1. red. now apply X.
+Qed.
+
+
   intros. destruct Σ as [Σ φ]. red in X0 |- *.
   simpl in *. induction X0; constructor; auto.
   clear IHX0. destruct d; simpl.
@@ -1238,13 +1336,13 @@ Definition type_local_decl `{checker_flags} Σ Γ d :=
 
 (** This predicate enforces that there exists typing derivations for every typable terms in env. *)
 
-Definition type_global_env `{checker_flags} (Σ : global_context) :=
+Definition type_global_env `{checker_flags} (Σ : global_env_ext) :=
   on_global_env (fun Σ => lift_typing typing Σ) Σ.
 
 (** ** Induction principle for typing up-to a global environment *)
 
 Definition Forall_decls_typing `{checker_flags}
-           (P : global_context -> context -> term -> term -> Type) : global_context -> Type :=
+           (P : global_env_ext -> context -> term -> term -> Type) : global_env_ext -> Type :=
   on_global_env (lift_typing P).
 
 Lemma refine_type `{checker_flags} Σ Γ t T U : Σ ;;; Γ |- t : T -> T = U -> Σ ;;; Γ |- t : U.
@@ -1253,8 +1351,8 @@ Proof. now intros Ht ->. Qed.
 Notation wf_local Σ Γ := (All_local_env (lift_typing typing Σ) Γ).
 
 Section wf_local_size.
-  Context `{checker_flags} (Σ : global_context).
-  Context (fn : forall (Σ : global_context) (Γ : context) (t T : term), typing Σ Γ t T -> size).
+  Context `{checker_flags} (Σ : global_env_ext).
+  Context (fn : forall (Σ : global_env_ext) (Γ : context) (t T : term), typing Σ Γ t T -> size).
 
   Fixpoint wf_local_size Γ (w : wf_local Σ Γ) : size :=
     match w with
@@ -1306,7 +1404,7 @@ Proof.
   induction d; simpl; try lia. destruct s as [s | [u Hu]]; try lia.
 Qed.
 
-Fixpoint globenv_size (Σ : global_declarations) : size :=
+Fixpoint globenv_size (Σ : global_env) : size :=
   match Σ with
   | [] => 1
   | d :: Σ => S (globenv_size Σ)
@@ -1314,7 +1412,7 @@ Fixpoint globenv_size (Σ : global_declarations) : size :=
 
 (** To get a good induction principle for typing derivations,
      we need:
-    - size of the global_context, including size of the global declarations in it
+    - size of the global_env_ext, including size of the global declarations in it
     - size of the derivation. *)
 
 Require Import Wf.
@@ -1325,22 +1423,32 @@ Require Import Wellfounded Relation_Definitions.
 Require Import Relation_Operators Lexicographic_Product Wf_nat.
 Arguments lexprod [A B].
 
-Notation wf := type_global_env.
+Definition wf := Forall_decls_typing typing.
+Definition wf_ext := on_global_env_ext (lift_typing typing).
 
 Definition env_prop `{checker_flags} (P : forall Σ Γ t T, Type) :=
-  forall Σ (wfΣ : wf Σ) Γ (wfΓ : wf_local Σ Γ) t T, Σ ;;; Γ |- t : T ->
+  forall Σ (wfΣ : wf Σ.1) Γ (wfΓ : wf_local Σ Γ) t T, Σ ;;; Γ |- t : T ->
     Forall_decls_typing P Σ * P Σ Γ t T.
 
 Lemma env_prop_typing `{checker_flags} P : env_prop P ->
-  forall Σ (wf : wf Σ) (Γ : context) (wfΓ : wf_local Σ Γ) (t T : term),
+  forall Σ (wf : wf Σ.1) (Γ : context) (wfΓ : wf_local Σ Γ) (t T : term),
     Σ ;;; Γ |- t : T -> P Σ Γ t T.
 Proof. intros. now apply X. Qed.
 
+Lemma type_Prop Σ : Σ ;;; [] |- tSort Universe.type0m : tSort Universe.type1.
+  repeat constructor.
+  apply prop_global_ext_levels.
+Defined.
+
+Definition empty_ext Σ : global_env_ext
+  := (Σ, Monomorphic_ctx ContextSet.empty).
+
 Lemma env_prop_sigma `{checker_flags} P : env_prop P ->
-  forall Σ (wf : wf Σ), Forall_decls_typing P Σ.
+  forall Σ (wf : wf Σ.1), Forall_decls_typing P Σ.
 Proof.
   intros. red in X. eapply X. apply wf. constructor. apply (type_Sort Σ [] Level.prop). constructor.
 Defined.
+
 
 Lemma wf_local_app `{checker_flags} Σ (Γ Γ' : context) : wf_local Σ (Γ ,,, Γ') -> wf_local Σ Γ.
 Proof.
@@ -1420,7 +1528,7 @@ Qed.
  *)
 (*
 Lemma typing_ind_env `{cf : checker_flags} :
-  forall (P : global_context -> context -> term -> term -> Type),
+  forall (P : global_env_ext -> context -> term -> term -> Type),
     (forall Σ (wfΣ : wf Σ) (Γ : context) (wfΓ : wf_local Σ Γ) (n : nat) decl,
         nth_error Γ n = Some decl -> All_local_env P Σ Γ ->
         P Σ Γ (tRel n) (lift0 (S n) decl.(decl_type))) ->
@@ -1465,19 +1573,19 @@ Lemma typing_ind_env `{cf : checker_flags} :
     (forall Σ (wfΣ : wf Σ) (Γ : context) (wfΓ : wf_local Σ Γ) (cst : ident) u (decl : constant_body),
         Forall_decls_typing P Σ ->
         All_local_env P Σ Γ ->
-        declared_constant (fst Σ) cst decl ->
+        declared_constant Σ.1 cst decl ->
         consistent_universe_context_instance Σ decl.(cst_universes) u ->
         P Σ Γ (tConst cst u) (subst_instance_constr u (cst_type decl))) ->
 
     (forall Σ (wfΣ : wf Σ) (Γ : context) (wfΓ : wf_local Σ Γ) (ind : inductive) u
-          mdecl idecl (isdecl : declared_inductive (fst Σ) mdecl ind idecl),
+          mdecl idecl (isdecl : declared_inductive Σ.1 mdecl ind idecl),
         Forall_decls_typing P Σ ->
         All_local_env P Σ Γ ->
         consistent_universe_context_instance Σ mdecl.(ind_universes) u ->
         P Σ Γ (tInd ind u) (subst_instance_constr u (ind_type idecl))) ->
 
     (forall Σ (wfΣ : wf Σ) (Γ : context) (wfΓ : wf_local Σ Γ) (ind : inductive) (i : nat) u
-            mdecl idecl cdecl (isdecl : declared_constructor (fst Σ) mdecl idecl (ind, i) cdecl),
+            mdecl idecl cdecl (isdecl : declared_constructor Σ.1 mdecl idecl (ind, i) cdecl),
         Forall_decls_typing P Σ ->
         All_local_env P Σ Γ ->
         consistent_universe_context_instance Σ mdecl.(ind_universes) u ->
@@ -1486,14 +1594,14 @@ Lemma typing_ind_env `{cf : checker_flags} :
     (forall Σ (wfΣ : wf Σ) (Γ : context) (wfΓ : wf_local Σ Γ) (ind : inductive) u (npar : nat)
             (p c : term) (brs : list (nat * term))
             (args : list term) (mdecl : mutual_inductive_body) (idecl : one_inductive_body)
-            (isdecl : declared_inductive (fst Σ) mdecl ind idecl),
+            (isdecl : declared_inductive Σ.1 mdecl ind idecl),
         Forall_decls_typing P Σ -> All_local_env P Σ Γ ->
         ind_npars mdecl = npar ->
         let pars := firstn npar args in
         forall (pty : term), Σ ;;; Γ |- p : pty -> P Σ Γ p pty ->
         forall indctx pctx ps btys,
         types_of_case ind mdecl idecl pars u p pty = Some (indctx, pctx, ps, btys) ->
-        check_correct_arity (snd Σ) idecl ind u indctx pars pctx = true ->
+        check_correct_arity (global_ext_constraints Σ) idecl ind u indctx pars pctx = true ->
         Exists (fun sf : sort_family => universe_family ps = sf) (ind_kelim idecl) ->
         P Σ Γ p pty ->
         Σ;;; Γ |- c : mkApps (tInd ind u) args ->
@@ -1503,7 +1611,7 @@ Lemma typing_ind_env `{cf : checker_flags} :
         P Σ Γ (tCase (ind, npar) p c brs) (mkApps p (skipn npar args ++ [c]))) ->
 
     (forall Σ (wfΣ : wf Σ) (Γ : context) (wfΓ : wf_local Σ Γ) (p : projection) (c : term) u
-          mdecl idecl pdecl (isdecl : declared_projection (fst Σ) mdecl idecl p pdecl) args,
+          mdecl idecl pdecl (isdecl : declared_projection Σ.1 mdecl idecl p pdecl) args,
         Forall_decls_typing P Σ -> All_local_env P Σ Γ ->
         Σ ;;; Γ |- c : mkApps (tInd (fst (fst p)) u) args ->
         P Σ Γ c (mkApps (tInd (fst (fst p)) u) args) ->
@@ -1542,7 +1650,7 @@ Proof.
   intros P X X0 X1 X2 X3 X4 X5 X6 X7 X8 X9 X10 X11 X12 Σ wfΣ Γ wfΓ t T H.
   pose (@Fix_F ({ Σ : _ & { wfΣ : wf Σ & { Γ : context & { wfΓ : wf_local Σ Γ &
                { t : term & { T : term & Σ ;;; Γ |- t : T }}}}}})
-               (lexprod (MR lt (fun Σ => globenv_size (fst Σ)))
+               (lexprod (MR lt (fun Σ => globenv_size Σ.1))
                             (fun Σ => MR lt (fun x => typing_size (projT2 (projT2 (projT2 (projT2 (projT2 x))))))))).
   set(foo := existT _ Σ (existT _ wfΣ (existT _ Γ (existT _ wfΓ (existT _ t (existT _ _ H))))) : { Σ : _ & { wfΣ : wf Σ & { Γ : context & { wfΓ & { t : term & { T : term & Σ ;;; Γ |- t : T }}}}}}).
   change Σ with (projT1 foo).
@@ -1680,7 +1788,7 @@ Proof.
     (*             typing_size Hty < *)
     (*             S *)
     (*               ((typing_spine_size *)
-    (*                   (fun (x : global_context) (x0 : context) (x1 x2 : term) (x3 : x;;; x0 |- x1 : x2) => *)
+    (*                   (fun (x : global_env_ext) (x0 : context) (x1 x2 : term) (x3 : x;;; x0 |- x1 : x2) => *)
     (*                      typing_size x3) Σ Γ t_ty l t' t0)) -> *)
     (*             Forall_decls_typing P Σ * P Σ Γ0 t1 T). *)
     (*    intros. unshelve eapply X14; eauto. lia. clear X14. clear n n0 H. *)
@@ -1731,7 +1839,7 @@ Proof.
                    S
                      (
                        (wf_local_size Σ
-                                      (fun (x : global_context) (x0 : context) (x1 x2 : term) (x3 : x;;; x0 |- x1 : x2) =>
+                                      (fun (x : global_env_ext) (x0 : context) (x1 x2 : term) (x3 : x;;; x0 |- x1 : x2) =>
                                          typing_size x3) Γ' a)) ->
                    Forall_decls_typing P Σ * P Σ Γ t T).
        intros; eauto. eapply (X14 _ X _ _ Hty); eauto. lia.
@@ -1773,7 +1881,7 @@ Proof.
                    S
                      (
                        (wf_local_size Σ
-                                      (fun (x : global_context) (x0 : context) (x1 x2 : term) (x3 : x;;; x0 |- x1 : x2) =>
+                                      (fun (x : global_env_ext) (x0 : context) (x1 x2 : term) (x3 : x;;; x0 |- x1 : x2) =>
                                          typing_size x3) Γ' a)) ->
 
                    Forall_decls_typing P Σ * P Σ Γ t T).
@@ -1816,7 +1924,7 @@ Definition env_prop_opt `{checker_flags} (P : forall Σ Γ t T, Type) :=
     Forall_decls_typing P Σ * P Σ Γ t T.
 
 Lemma typing_ind_env `{cf : checker_flags} :
-  forall (P : global_context -> context -> term -> term -> Type)
+  forall (P : global_env_ext -> context -> term -> term -> Type)
          (Pdecl := fun Σ Γ wfΓ t T tyT => P Σ Γ t T),
     (forall Σ (wfΣ : wf Σ) (Γ : context) (wfΓ : wf_local Σ Γ) (n : nat) decl,
         nth_error Γ n = Some decl ->
@@ -1863,35 +1971,35 @@ Lemma typing_ind_env `{cf : checker_flags} :
     (forall Σ (wfΣ : wf Σ) (Γ : context) (wfΓ : wf_local Σ Γ) (cst : ident) u (decl : constant_body),
         Forall_decls_typing P Σ ->
         All_local_env_over typing Pdecl Σ Γ wfΓ ->
-        declared_constant (fst Σ) cst decl ->
-        consistent_universe_context_instance (snd Σ) decl.(cst_universes) u ->
+        declared_constant Σ.1 cst decl ->
+        consistent_instance_ext Σ decl.(cst_universes) u ->
         P Σ Γ (tConst cst u) (subst_instance_constr u (cst_type decl))) ->
 
     (forall Σ (wfΣ : wf Σ) (Γ : context) (wfΓ : wf_local Σ Γ) (ind : inductive) u
-          mdecl idecl (isdecl : declared_inductive (fst Σ) mdecl ind idecl),
+          mdecl idecl (isdecl : declared_inductive Σ.1 mdecl ind idecl),
         Forall_decls_typing P Σ ->
         All_local_env_over typing Pdecl Σ Γ wfΓ ->
-        consistent_universe_context_instance (snd Σ) mdecl.(ind_universes) u ->
+        consistent_instance_ext Σ mdecl.(ind_universes) u ->
         P Σ Γ (tInd ind u) (subst_instance_constr u (ind_type idecl))) ->
 
     (forall Σ (wfΣ : wf Σ) (Γ : context) (wfΓ : wf_local Σ Γ) (ind : inductive) (i : nat) u
-            mdecl idecl cdecl (isdecl : declared_constructor (fst Σ) mdecl idecl (ind, i) cdecl),
+            mdecl idecl cdecl (isdecl : declared_constructor Σ.1 mdecl idecl (ind, i) cdecl),
         Forall_decls_typing P Σ ->
         All_local_env_over typing Pdecl Σ Γ wfΓ ->
-        consistent_universe_context_instance (snd Σ) mdecl.(ind_universes) u ->
+        consistent_instance_ext Σ mdecl.(ind_universes) u ->
         P Σ Γ (tConstruct ind i u) (type_of_constructor mdecl cdecl (ind, i) u)) ->
 
     (forall Σ (wfΣ : wf Σ) (Γ : context) (wfΓ : wf_local Σ Γ) (ind : inductive) u (npar : nat)
             (p c : term) (brs : list (nat * term))
             (args : list term) (mdecl : mutual_inductive_body) (idecl : one_inductive_body)
-            (isdecl : declared_inductive (fst Σ) mdecl ind idecl),
+            (isdecl : declared_inductive Σ.1 mdecl ind idecl),
         Forall_decls_typing P Σ -> All_local_env_over typing Pdecl Σ Γ wfΓ ->
         ind_npars mdecl = npar ->
         let pars := firstn npar args in
         forall (pty : term), Σ ;;; Γ |- p : pty ->
         forall indctx pctx ps btys,
         types_of_case ind mdecl idecl pars u p pty = Some (indctx, pctx, ps, btys) ->
-        check_correct_arity (snd Σ) idecl ind u indctx pars pctx ->
+        check_correct_arity (global_ext_constraints Σ) idecl ind u indctx pars pctx ->
         Exists (fun sf : sort_family => universe_family ps = sf) (ind_kelim idecl) ->
         P Σ Γ p pty ->
         Σ;;; Γ |- c : mkApps (tInd ind u) args ->
@@ -1901,7 +2009,7 @@ Lemma typing_ind_env `{cf : checker_flags} :
         P Σ Γ (tCase (ind, npar) p c brs) (mkApps p (skipn npar args ++ [c]))) ->
 
     (forall Σ (wfΣ : wf Σ) (Γ : context) (wfΓ : wf_local Σ Γ) (p : projection) (c : term) u
-          mdecl idecl pdecl (isdecl : declared_projection (fst Σ) mdecl idecl p pdecl) args,
+          mdecl idecl pdecl (isdecl : declared_projection Σ.1 mdecl idecl p pdecl) args,
         Forall_decls_typing P Σ -> All_local_env_over typing Pdecl Σ Γ wfΓ ->
         Σ ;;; Γ |- c : mkApps (tInd (fst (fst p)) u) args ->
         P Σ Γ c (mkApps (tInd (fst (fst p)) u) args) ->
@@ -1942,7 +2050,7 @@ Proof.
   intros X X0 X1 X2 X3 X4 X5 X6 X7 X8 X9 X10 X11 X12 Σ wfΣ Γ wfΓ t T H.
   pose (@Fix_F ({ Σ : _ & { wfΣ : wf Σ & { Γ : context & { wfΓ : wf_local Σ Γ &
                { t : term & { T : term & Σ ;;; Γ |- t : T }}}}}})
-               (lexprod (MR lt (fun Σ => globenv_size (fst Σ)))
+               (lexprod (MR lt (fun Σ => globenv_size Σ.1))
                             (fun Σ => MR lt (fun x => typing_size (projT2 (projT2 (projT2 (projT2 (projT2 x))))))))).
   set(foo := existT _ Σ (existT _ wfΣ (existT _ Γ (existT _ wfΓ (existT _ t (existT _ _ H))))) : { Σ : _ & { wfΣ : wf Σ & { Γ : context & { wfΓ & { t : term & { T : term & Σ ;;; Γ |- t : T }}}}}}).
   change Σ with (projT1 foo).
@@ -2132,7 +2240,7 @@ Proof.
                  forall (t T : term) (Hty : Σ;;; Γ |- t : T),
                    typing_size Hty <
                    S ((wf_local_size Σ
-                       (fun (x : global_context) (x0 : context) (x1 x2 : term) (x3 : x;;; x0 |- x1 : x2) =>
+                       (fun (x : global_env_ext) (x0 : context) (x1 x2 : term) (x3 : x;;; x0 |- x1 : x2) =>
                           typing_size x3) Γ' a)) ->
                    Forall_decls_typing P Σ * P Σ Γ t T).
        intros; eauto. eapply (X14 _ X _ _ Hty); eauto. lia.
@@ -2181,7 +2289,7 @@ Proof.
                    S
                      (
                        (wf_local_size Σ
-                                      (fun (x : global_context) (x0 : context) (x1 x2 : term) (x3 : x;;; x0 |- x1 : x2) =>
+                                      (fun (x : global_env_ext) (x0 : context) (x1 x2 : term) (x3 : x;;; x0 |- x1 : x2) =>
                                          typing_size x3) Γ' a)) ->
 
                    Forall_decls_typing P Σ * P Σ Γ t T).
@@ -2264,7 +2372,7 @@ Qed.
 
 Lemma lookup_on_global_env `{checker_flags} P Σ c decl :
   on_global_env P Σ ->
-  lookup_env (fst Σ) c = Some decl ->
+  lookup_env Σ.1 c = Some decl ->
   { Σ' & { wfΣ' : on_global_env P Σ' & on_global_decl P Σ' decl } }.
 Proof.
   induction 1; simpl. congruence.
@@ -2322,7 +2430,7 @@ Proof.
 Qed.
 
 Definition property `{checker_flags} :=
-  forall (Σ : global_context) (Γ : context),
+  forall (Σ : global_env_ext) (Γ : context),
     All_local_env (lift_typing typing Σ) Γ -> forall t T : term, typing Σ Γ t T -> Type.
 
 Definition lookup_wf_local {Γ P} (wfΓ : All_local_env P Γ) (n : nat) (isdecl : n < #|Γ|) :
