pcuic/theories/PCUICMetaTheory.v
@@ -9,20 +9,16 @@ Set Asymmetric Patterns.
 
 Existing Instance config.default_checker_flags.
 
-(** Use a coercion for this common projection of the global context. *)
-Definition fst_ctx : global_context -> global_declarations := fst.
-Coercion fst_ctx : global_context >-> global_declarations.
-
 (** The subject reduction property of the system: *)
 
 (* Commented otherwise extraction would produce an axiom making the whole
    extracted code unusable *)
-(* Conjecture subject_reduction : forall (Σ : global_context) Γ t u T, *)
+(* Conjecture subject_reduction : forall (Σ : global_env_ext) Γ t u T, *)
 (*     Σ ;;; Γ |- t : T -> red Σ Γ t u -> Σ ;;; Γ |- u : T. *)
 
 (** Weak Normalization: every term has a normal form *)
 
-Definition normal (Σ : global_context) Γ t := { u : _ & red1 Σ Γ t u } -> False.
+Definition normal (Σ : global_env_ext) Γ t := { u : _ & red1 Σ Γ t u } -> False.
 
-Conjecture weak_normalization : forall (Σ : global_context) Γ t T,
+Conjecture weak_normalization : forall (Σ : global_env_ext) Γ t T,
     Σ ;;; Γ |- t : T -> { u & (red Σ Γ t u * normal Σ Γ u)%type }.
